proof/DDC/Language/SystemF2Data/Progress.v
@@ -1,0 +1,158 @@
+
+Require Import DDC.Language.SystemF2Data.Step.
+Require Import DDC.Language.SystemF2Data.TyJudge.
+Require Import DDC.Language.SystemF2Data.Exp.
+Require Import DDC.Base.
+
+
+(* A well typed expression is either a well formed value, 
+   or can transition to the next state. *)
+Theorem progress
+ :  forall ds x t
+ ,  DEFSOK ds
+ -> TYPE ds nil nil x t
+ -> value x \/ (exists x', STEP x x').
+Proof.
+ intros. gen t.
+ induction x using exp_mutind with 
+  (PA := fun a => a = a)
+  ; intros.
+
+
+ Case "XVar".
+  nope.
+
+
+ Case "XLAM".
+  left. apply type_wfX in H0. auto.
+
+
+ Case "XAPP".
+  inverts keep H0.
+  edestruct IHx. eauto.
+  SCase "x value".
+   right. inverts H1. inverts H3.
+    SSCase "x = XVar". nope.
+    SSCase "x = XLAM". exists (substTX 0 t2 x1). eapply ESLAMAPP.
+    SSCase "x = XAPP". nope.
+    SSCase "x = XApp". nope.
+
+    SSCase "x = XCon".
+     (* TODO: XAPP (XCon dc tsParam xs) t2) cant happen as it's miskinded.
+              need lemma saying kind of value types is KStar *)
+     skip.
+
+    SSCase "x = XCase".
+     nope.
+  SCase "x steps".
+   right.
+    dest x'.
+    exists (XAPP x' t2).
+    lets D: EsContext XcAPP H1.
+    eauto.
+
+
+ Case "XLam".
+  left. eapply type_wfX in H0. auto.
+
+
+ Case "XApp".
+  right.
+  inverts_type.
+  edestruct IHx1; eauto.
+  SCase "value x1".
+   edestruct IHx2; eauto.
+    SSCase "value x2".
+     assert (exists t x, x1 = XLam t x) as HF. eauto.
+     destruct HF as [t11].
+     destruct H2 as [x12].
+     subst.
+     exists (substXX 0 x2 x12). 
+     apply EsLamApp; eauto.
+    SSCase "x2 steps".
+     destruct H1 as [x2'].
+     exists (XApp x1 x2'). auto.
+  SCase "x1 steps".
+   destruct H0  as [x1'].
+   exists (XApp x1' x2).
+   eapply (EsContext (fun xx => XApp xx x2)); auto.
+ 
+
+ Case "XCon".
+  inverts_type.
+  (* All ctor args are either wnf or can step *)
+  assert (Forall (fun x => wnfX x \/ (exists x', STEP x x')) xs) as HWS.
+   nforall. intros.
+   assert (exists t, TYPE ds nil nil x t).
+    eapply Forall2_exists_left; eauto.
+    dest t.
+   assert (value x \/ (exists x', STEP x x')).
+    eapply H0; eauto.
+   int.     
+
+  (* All ctor args are wnf, or there is a context where one can step *)
+  lets D: (@exps_ctx_run exp exp) HWS.
+  inverts D.
+   (* All ctor args are wnf *)
+   left.
+   assert (Forall (wfT 0) ts).   eauto. admit. (* ok ts WK under nil*)
+   assert (Forall (wfX 0 0) xs). eauto. admit. (* ok xs WT under nil nil *)
+   eauto. 
+
+   (* There is a context where one ctor arg can step *)
+   right.
+    dest C. dest x'.
+    int. subst.
+    lets D: step_context_XCon_exists H2 H4.
+    destruct D as [x'']. eauto.
+
+
+ Case "XCase".
+  right.
+  inverts keep H1.
+  assert (value x \/ (exists x', STEP x x')) as HS; eauto.
+  inverts HS. clear IHx.
+  SCase "x value".
+   destruct x; nope.
+    SSCase "XCase (XLAM x) aa".
+     assert (exists t', tObj = TForall t'). eauto.
+     dest t'. subst.
+     false.
+
+    SSCase "XCase (XLam t x) aa".
+     assert (exists t11 t12, tObj = tFun t11 t12). eauto.
+     dest t11. dest t12. subst.
+     unfold tFun in H6. 
+     simpl in H6. inverts H6.
+     assert (DEFOK ds (DefDataType TyConFun ks dcs)). eauto.
+      inverts H3. false.
+
+    SSCase "XCon".
+     (* show there is a corresponding alternative 
+        TODO: split this into a lemma *)
+     assert (exists x, getAlt d aa = Some (AAlt d x)) as HG.
+      eapply getAlt_exists.
+      nforall.
+      eapply H9. 
+      inverts H4.
+
+      assert (getCtorOfType (TCon tc) = Some tc). auto.
+      erewrite getCtorOfType_makeTApps in H6; eauto.
+       inverts H6.
+      eauto.
+
+     dest x.
+     exists (substXXs 0 l0 x).
+     eapply EsCaseAlt; eauto.
+
+  SCase "x steps".
+   destruct H2 as [x'].
+   exists (XCase x' aa).
+   lets D: EsContext XcCase; eauto.
+
+
+ Case "XAlt".
+   auto.     
+Qed.
+
+
